Add axiom to correlate reveal_ constants for overrides

Source/DafnyCore/Verifier/BoogieGenerator.cs
@@ -1042,6 +1042,14 @@ namespace Microsoft.Dafny {
         sink.AddTopLevelDeclaration(revealTrigger);
         Bpl.Expr revealTrigger_expr = new Bpl.IdentifierExpr(f.tok, revealTrigger);
         this.functionReveals[f] = revealTrigger_expr;
+
+        // If this is an override, generate:
+        //     axiom reveal_FunctionA ==> reveal_FunctionParent;
+        if (f.OverriddenFunction is { IsOpaque: true }) {
+          var revealParent = GetRevealConstant(f.OverriddenFunction);
+          var implication = BplImp(revealTrigger_expr, revealParent);
+          AddOtherDefinition(revealTrigger, new Axiom(f.tok, implication));
+        }
       }
     }
 
